Require dtm on after_external & do house keeping

x86/AsmregsC.v
@@ -173,3 +173,126 @@ Inductive load_arguments (rs_arg: regset) (m_arg: mem) (sg_init: signature)
     (DROP: Mem_set_perm m_arg sp 0 (4 * (size_arguments sg_init)) None = Some m_init)
 .
 
+
+
+Definition to_preg := preg_of.
+
+Definition to_mreg (pr: preg): option mreg :=
+  match pr with
+  | PC => None
+  | ST0 => Some FP0
+  | CR _ => None
+  | RA => None
+  | IR ir =>
+    match ir with
+    | RAX => Some AX
+    | RBX => Some BX
+    | RCX => Some CX
+    | RDX => Some DX
+    | RSI => Some SI
+    | RDI => Some DI
+    | RBP => Some BP
+    | RSP => None
+    | R8 => Some Machregs.R8
+    | R9 => Some Machregs.R9
+    | R10 => Some Machregs.R10
+    | R11 => Some Machregs.R11
+    | R12 => Some Machregs.R12
+    | R13 => Some Machregs.R13
+    | R14 => Some Machregs.R14
+    | R15 => Some Machregs.R15
+    end
+  | FR fr =>
+    match fr with
+    | XMM0 => Some X0
+    | XMM1 => Some X1
+    | XMM2 => Some X2
+    | XMM3 => Some X3
+    | XMM4 => Some X4
+    | XMM5 => Some X5
+    | XMM6 => Some X6
+    | XMM7 => Some X7
+    | XMM8 => Some X8
+    | XMM9 => Some X9
+    | XMM10 => Some X10
+    | XMM11 => Some X11
+    | XMM12 => Some X12
+    | XMM13 => Some X13
+    | XMM14 => Some X14
+    | XMM15 => Some X15
+    end
+  end
+.
+
+Lemma to_preg_to_mreg
+      mr0
+  :
+    mr0.(to_preg).(to_mreg) = Some mr0
+.
+Proof.
+  destruct mr0; ss.
+Qed.
+
+Lemma to_mreg_injective
+      pr0 pr1
+      (SOME: is_some (pr0.(to_mreg)))
+      (EQ: pr0.(to_mreg) = pr1.(to_mreg))
+  :
+    <<EQ: pr0 = pr1>>
+.
+Proof.
+  destruct pr0; ss; destruct pr1; ss; des_ifs.
+Qed.
+
+Lemma preg_of_injective
+      mr0 mr1
+      (EQ: preg_of mr0 = preg_of mr1)
+  :
+    <<EQ: mr0 = mr1>>
+.
+Proof. destruct mr0, mr1; ss. Qed.
+
+Lemma to_mreg_to_preg
+      pr0
+  :
+    o_map (pr0.(to_mreg)) (to_preg) = Some pr0 \/ pr0.(to_mreg) = None
+.
+Proof.
+  destruct pr0; ss; des_ifs; eauto.
+Qed.
+
+Corollary to_mreg_some_to_preg
+      pr0 mr0
+      (SOME: pr0.(to_mreg) = Some mr0)
+  :
+    <<EQ: mr0.(to_preg) = pr0>>
+.
+Proof.
+  eapply to_mreg_injective with (pr0 := mr0.(to_preg)) (pr1 := pr0).
+  { rewrite to_preg_to_mreg; ss. }
+  rewrite to_preg_to_mreg; ss.
+Qed.
+
+Print Conventions1.
+(* Note: callee_save registers all reside in mregs. So we can just put undef on preg\mreg. *)
+
+Inductive is_callee_save (sg: signature) (pr: preg): Prop :=
+| is_callee_save_some
+    mr
+    (MREG: pr.(to_mreg) = Some mr)
+    (CALLEESAVE: Conventions1.is_callee_save mr)
+| is_callee_save_none
+    (MREG: pr.(to_mreg) = None)
+.
+
+Inductive callee_saved (sg: signature) (rs0 rs1: regset): Prop :=
+| callee_saved_intro
+    (TODO: True)
+    (CALLEESAVE: forall
+        r
+        (CALLEESAVE: is_callee_save sg r)
+      ,
+        <<SAVE: Val.lessdef (rs0 r) (rs1 r)>>)
+(* In Compcert' sg is not needed (see is_callee_save). Is it true in real-world too? *)
+.
+
